[Civl] List refactor (#1120)

Test/civl/large-samples/treiber-stack.bpl
@@ -14,10 +14,6 @@ function {:inline} Domain(ts: Map (One Loc) (Treiber X), loc_t: Loc): [One Loc]b
   ts->val[One(loc_t)]->nodes->dom
 }
 
-function {:inline} ListInDomain(t: Treiber X): bool {
-  (forall x: Loc:: BetweenSet(t->nodes->val, t->top, None())[x] ==> Set_Contains(t->nodes->dom, One(x)))
-}
-
 yield invariant {:layer 1} TopInStack(loc_t: Loc);
 preserves Map_Contains(TreiberPoolLow, One(loc_t));
 preserves (var loc_n := Map_At(TreiberPoolLow, One(loc_t))->top; loc_n is None || Set_Contains(Domain(TreiberPoolLow, loc_t), One(loc_n->t)));
@@ -32,9 +28,9 @@ preserves loc_n is None || Set_Contains(Domain(TreiberPoolLow, loc_t), One(loc_n
 yield invariant {:layer 2} ReachInStack(loc_t: Loc);
 preserves Map_Contains(TreiberPoolLow, One(loc_t));
 preserves (var t := Map_At(TreiberPoolLow, One(loc_t)); Between(t->nodes->val, t->top, t->top, None()));
-preserves (var t := Map_At(TreiberPoolLow, One(loc_t)); ListInDomain(t));
+preserves (var t := Map_At(TreiberPoolLow, One(loc_t)); ListInDomain(t->top, t->nodes));
 preserves (var loc_n := Map_At(TreiberPoolLow, One(loc_t))->top; loc_n is None || Set_Contains(Domain(TreiberPoolLow, loc_t), One(loc_n->t)));
-preserves Map_At(TreiberPool, One(loc_t)) == Abs(Map_At(TreiberPoolLow, One(loc_t)));
+preserves (var t := Map_At(TreiberPoolLow, One(loc_t)); Map_At(TreiberPool, One(loc_t)) == StackAbs(t->top, t->nodes));
 
 yield invariant {:layer 2} StackDom();
 preserves TreiberPool->dom == TreiberPoolLow->dom;
@@ -71,9 +67,9 @@ preserves call StackDom();
   call stack := Map_MakeEmpty();
   treiber := Treiber(top, stack);
   call one_loc_t, tag := Tag_New();
-  call AllocTreiber#0(one_loc_t, treiber);
+  call AllocTreiber(one_loc_t, treiber);
   call {:layer 2} TreiberPool := Copy(Map_Update(TreiberPool, one_loc_t, Vec_Empty()));
-  call {:layer 2} AbsLemma(treiber);
+  call {:layer 2} StackAbsLemma(treiber->top, treiber->nodes);
 }
 
 atomic action {:layer 3} AtomicPush(loc_t: Loc, x: X) returns (success: bool)
@@ -85,7 +81,7 @@ atomic action {:layer 3} AtomicPush(loc_t: Loc, x: X) returns (success: bool)
     success := false;
   }
 }
-yield procedure {:layer 2} {:vcs_split_on_every_assert} Push(loc_t: Loc, x: X) returns (success: bool)
+yield procedure {:layer 2} Push(loc_t: Loc, x: X) returns (success: bool)
 refines AtomicPush;
 preserves call TopInStack(loc_t);
 preserves call ReachInStack(loc_t);
@@ -94,19 +90,20 @@ preserves call StackDom();
   var old_top: Option Loc;
   var new_top: Loc;
   var tag: One (Tag Unit);
-  var {:layer 2} old_treiber: Treiber X;
+  var {:layer 2} old_treiber, mid_treiber, new_treiber: Treiber X;
 
   call {:layer 2} old_treiber := Copy(TreiberPoolLow->val[One(loc_t)]);
-  call old_top, tag := AllocNode#1(loc_t, x);
+  call old_top, tag := AddNode(loc_t, x);
+  call {:layer 2} mid_treiber := Copy(TreiberPoolLow->val[One(loc_t)]);
+  call {:layer 2} StackFrameLemma(old_treiber->top, old_treiber->nodes, mid_treiber->nodes);
   new_top := tag->val->loc;
-  call {:layer 2} FrameLemma(old_treiber, TreiberPoolLow->val[One(loc_t)]);
   call ReachInStack(loc_t) | StackDom() | PushLocInStack(loc_t, new_top, Node(old_top, x), tag);
-  call success := WriteTopOfStack#0(loc_t, old_top, Some(new_top));
+  call success := WriteTopOfStack(loc_t, old_top, Some(new_top));
   if (success) {
+    call {:layer 2} new_treiber := Copy(TreiberPoolLow->val[One(loc_t)]);
     assert {:layer 2} Map_Contains(TreiberPool, One(loc_t));
     call {:layer 2} TreiberPool := Copy(Map_Update(TreiberPool, One(loc_t), Vec_Append(Map_At(TreiberPool, One(loc_t)), x)));
-    assert {:layer 2} TreiberPoolLow->val[One(loc_t)]->top != None();
-    call {:layer 2} AbsLemma(TreiberPoolLow->val[One(loc_t)]);
+    call {:layer 2} StackAbsLemma(new_treiber->top, new_treiber->nodes);
   }
 }
 
@@ -134,7 +131,10 @@ preserves call TopInStack(loc_t);
 preserves call ReachInStack(loc_t);
 preserves call StackDom();
 {
-  call {:layer 2} AbsLemma(TreiberPoolLow->val[One(loc_t)]);
+  var {:layer 2} treiber: Treiber X;
+
+  call {:layer 2} treiber := Copy(TreiberPoolLow->val[One(loc_t)]);
+  call {:layer 2} StackAbsLemma(treiber->top, treiber->nodes);
   call success, x_opt := PopIntermediate(loc_t);
   if (x_opt is Some) {
     assert {:layer 2} Vec_Len(Map_At(TreiberPool, One(loc_t))) > 0;
@@ -142,7 +142,7 @@ preserves call StackDom();
   }
 }
 
-atomic action {:layer 2} AtomicAllocNode#1(loc_t: Loc, x: X)
+atomic action {:layer 2} AtomicAddNode(loc_t: Loc, x: X)
   returns (old_top: Option Loc, {:linear} tag: One (Tag Unit))
 asserts Map_Contains(TreiberPoolLow, One(loc_t));
 {
@@ -161,18 +161,18 @@ asserts Map_Contains(TreiberPoolLow, One(loc_t));
   treiber := Treiber(top, stack);
   call Map_Put(TreiberPoolLow, one_loc_t, treiber);
 }
-yield procedure {:layer 1} AllocNode#1(loc_t: Loc, x: X)
+yield procedure {:layer 1} AddNode(loc_t: Loc, x: X)
   returns (old_top: Option Loc, {:linear} tag: One (Tag Unit))
 preserves call TopInStack(loc_t);
 ensures call LocInStackOrNone(loc_t, Some(tag->val->loc));
-refines AtomicAllocNode#1;
+refines AtomicAddNode;
 {
   var one_loc_n: One Loc;
 
-  call old_top := ReadTopOfStack#0(loc_t);
+  call old_top := ReadTopOfStack(loc_t);
   call LocInStackOrNone(loc_t, old_top) | TopInStack(loc_t);
   call one_loc_n, tag := Tag_New();
-  call AllocNode#0(loc_t, one_loc_n, Node(old_top, x));
+  call AllocNode(loc_t, one_loc_n, Node(old_top, x));
 }
 
 atomic action {:layer 2} AtomicPopIntermediate(loc_t: Loc) returns (success: bool, x_opt: Option X)
@@ -213,16 +213,16 @@ preserves call TopInStack(loc_t);
   var node: Node X;
   var x: X;
 
-  call loc_n := ReadTopOfStack#0(loc_t);
+  call loc_n := ReadTopOfStack(loc_t);
   if (loc_n == None()) {
     x_opt := None();
     success := true;
     return;
   }
   call LocInStackOrNone(loc_t, loc_n) | TopInStack(loc_t);
-  call node := LoadNode#0(loc_t, loc_n->t);
+  call node := LoadNode(loc_t, loc_n->t);
   Node(new_loc_n, x) := node;
-  call success := WriteTopOfStack#0(loc_t, loc_n, new_loc_n);
+  call success := WriteTopOfStack(loc_t, loc_n, new_loc_n);
   if (success) {
     x_opt := Some(x);
   } else {
@@ -232,19 +232,19 @@ preserves call TopInStack(loc_t);
 
 /// Primitives
 
-yield procedure {:layer 0} LoadNode#0(loc_t: Loc, loc_n: Loc) returns (node: Node X);
+yield procedure {:layer 0} LoadNode(loc_t: Loc, loc_n: Loc) returns (node: Node X);
 refines right action {:layer 1} _
 {
   call node := Path_Load(TreiberPoolLow->val[One(loc_t)]->nodes->val[One(loc_n)]);
 }
 
-yield procedure {:layer 0} ReadTopOfStack#0(loc_t: Loc) returns (loc_n: Option Loc);
+yield procedure {:layer 0} ReadTopOfStack(loc_t: Loc) returns (loc_n: Option Loc);
 refines atomic action {:layer 1} _
 {
   call loc_n := Path_Load(TreiberPoolLow->val[One(loc_t)]->top);
 }
 
-yield procedure {:layer 0} WriteTopOfStack#0(
+yield procedure {:layer 0} WriteTopOfStack(
   loc_t: Loc, old_loc_n: Option Loc, new_loc_n: Option Loc) returns (success: bool);
 refines atomic action {:layer 1,2} _
 {
@@ -258,79 +258,14 @@ refines atomic action {:layer 1,2} _
   }
 }
 
-yield procedure {:layer 0} AllocNode#0(loc_t: Loc, {:linear_in} one_loc_n: One Loc, node: Node X);
+yield procedure {:layer 0} AllocNode(loc_t: Loc, {:linear_in} one_loc_n: One Loc, node: Node X);
 refines atomic action {:layer 1} _
 {
   call Map_Put(TreiberPoolLow->val[One(loc_t)]->nodes, one_loc_n, node);
 }
 
-yield procedure {:layer 0} AllocTreiber#0({:linear_in} one_loc_t: One Loc, {:linear_in} treiber: Treiber X);
+yield procedure {:layer 0} AllocTreiber({:linear_in} one_loc_t: One Loc, {:linear_in} treiber: Treiber X);
 refines atomic action {:layer 1,2} _
 {
   call Map_Put(TreiberPoolLow, one_loc_t, treiber);
-}
-
-/// Proof of abstraction with a manual encoding of termination
-
-// Abs and AbsDefinition together model the abstraction function
-function Abs(treiber: Treiber X): Vec X;
-function {:inline} AbsDefinition(treiber: Treiber X): Vec X {
-if treiber->top == None() then
-  Vec_Empty() else
-  (var n := Map_At(treiber->nodes, One(treiber->top->t));
-    (var treiber' := Treiber(n->next, treiber->nodes); 
-      Vec_Append(Abs(treiber'), n->val)))
-}
-
-pure procedure AbsCompute(treiber: Treiber X, treiber': Treiber X) returns (absStack: Vec X)
-requires treiber->top == treiber'->top;
-requires Set_IsSubset(treiber->nodes->dom, treiber'->nodes->dom);
-requires MapIte(treiber->nodes->dom, treiber->nodes->val, MapConst(Default())) ==
-         MapIte(treiber->nodes->dom, treiber'->nodes->val, MapConst(Default()));
-requires Between(treiber->nodes->val, treiber->top, treiber->top, None());
-requires ListInDomain(treiber);
-ensures absStack == AbsDefinition(treiber);
-ensures absStack == AbsDefinition(treiber');
-free ensures absStack == Abs(treiber);
-free ensures absStack == Abs(treiber');
-{
-  var loc_n: Option Loc;
-  var n: Node X;
-
-  if (treiber->top == None()) {
-      absStack := Vec_Empty();
-  } else {
-      loc_n := treiber->top;
-      assert Map_Contains(treiber->nodes, One(loc_n->t));
-      n := Map_At(treiber->nodes, One(loc_n->t));
-      // Use well-founded list reachability to prove that recursion will terminate:
-      // treiber@caller->top --> treiber@callee->top --> None()
-      assert Between(treiber->nodes->val, loc_n, n->next, None());
-      call absStack := AbsCompute(Treiber(n->next, treiber->nodes), Treiber(n->next, treiber'->nodes));
-      absStack := Vec_Append(absStack, n->val);
-  }
-}
-
-/// Useful lemmas obtained by wrapping AbsCompute
-
-pure procedure AbsLemma(treiber: Treiber X)
-requires Between(treiber->nodes->val, treiber->top, treiber->top, None());
-requires ListInDomain(treiber);
-ensures Abs(treiber) == AbsDefinition(treiber);
-{
-  var absStack: Vec X;
-  call absStack := AbsCompute(treiber, treiber);
-}
-
-pure procedure FrameLemma(treiber: Treiber X, treiber': Treiber X)
-requires treiber->top == treiber'->top;
-requires Set_IsSubset(treiber->nodes->dom, treiber'->nodes->dom);
-requires MapIte(treiber->nodes->dom, treiber->nodes->val, MapConst(Default())) ==
-         MapIte(treiber->nodes->dom, treiber'->nodes->val, MapConst(Default()));
-requires Between(treiber->nodes->val, treiber->top, treiber->top, None());
-requires ListInDomain(treiber);
-ensures Abs(treiber) == Abs(treiber');
-{
-  var absStack: Vec X;
-  call absStack := AbsCompute(treiber, treiber');
 }
